feat: Use ESDKEncryptedDataKey[s]

src/SDK/MessageHeader.dfy
@@ -8,10 +8,10 @@ include "Materials.dfy"
 include "../Util/UTF8.dfy"
 include "../Util/Sets.dfy"
 include "../Crypto/AESEncryption.dfy"
-include "../Generated/AwsCryptographicMaterialProviders.dfy"
+include "Serialize/SerializableTypes.dfy"
 
 module {:extern "MessageHeader"} MessageHeader {
-  import Aws.Crypto
+  import opened SerializableTypes
   import AlgorithmSuite
   import Sets
   import opened Wrappers
@@ -73,28 +73,19 @@ module {:extern "MessageHeader"} MessageHeader {
   {
   }
 
-  datatype EncryptedDataKeys = EncryptedDataKeys(entries: seq<Crypto.EncryptedDataKey>)
-  {
-    predicate Valid() {
-      && 0 < |entries| < UINT16_LIMIT
-      && (forall i :: 0 <= i < |entries| ==> entries[i].Valid())
-    }
-  }
-
   datatype HeaderBody = HeaderBody(
                           version: Version,
                           typ: Type,
                           algorithmSuiteID: AlgorithmSuite.ID,
                           messageID: MessageID,
                           aad: EncryptionContext.Map,
-                          encryptedDataKeys: EncryptedDataKeys,
+                          encryptedDataKeys: ESDKEncryptedDataKeys,
                           contentType: ContentType,
                           ivLength: uint8,
                           frameLength: uint32)
   {
     predicate Valid() {
       && EncryptionContext.Serializable(aad)
-      && encryptedDataKeys.Valid()
       && algorithmSuiteID.IVLength() == ivLength as nat
       && ValidFrameLength(frameLength, contentType)
     }
@@ -141,40 +132,23 @@ module {:extern "MessageHeader"} MessageHeader {
     UInt32ToSeq(hb.frameLength)
   }
 
-  function EDKsToSeq(encryptedDataKeys: EncryptedDataKeys): seq<uint8>
-    requires encryptedDataKeys.Valid()
+  function EDKsToSeq(encryptedDataKeys: ESDKEncryptedDataKeys): seq<uint8>
   {
-    var n := |encryptedDataKeys.entries|;
+    var n := |encryptedDataKeys|;
     UInt16ToSeq(n as uint16) +
-    EDKEntriesToSeq(encryptedDataKeys.entries, 0, n)
+    EDKEntriesToSeq(encryptedDataKeys, 0, n)
   }
 
-  function EDKEntriesToSeq(entries: seq<Crypto.EncryptedDataKey>, lo: nat, hi: nat): seq<uint8>
-    requires forall i :: 0 <= i < |entries| ==> entries[i].Valid()
+  function EDKEntriesToSeq(entries: ESDKEncryptedDataKeys, lo: nat, hi: nat): seq<uint8>
     requires lo <= hi <= |entries|
   {
-    if lo == hi then [] else EDKEntriesToSeq(entries, lo, hi - 1) + EDKEntryToSeq(entries[hi - 1])
+    if lo == hi then
+      []
+    else
+      EDKEntriesToSeq(entries, lo, hi - 1) + EDKEntryToSeq(entries[hi - 1])
   }
 
-  lemma EDKEntriesToSeqInductiveStep(entriesHead: seq<Crypto.EncryptedDataKey>, entriesTail: seq<Crypto.EncryptedDataKey>, lo: nat, hi: nat)
-    requires var entries := entriesHead + entriesTail;
-      forall i :: 0 <= i < |entries| ==> (entries)[i].Valid()
-    requires lo <= hi <= |entriesHead|
-    ensures forall i :: 0 <= i < |entriesHead| ==> entriesHead[i].Valid()
-    ensures var entries := entriesHead + entriesTail;
-      EDKEntriesToSeq(entriesHead + entriesTail, lo, hi) == EDKEntriesToSeq(entriesHead, lo, hi)
-  {
-    assert forall i :: 0 <= i < |entriesHead| ==> entriesHead[i].Valid() by {
-      if !(forall i :: 0 <= i < |entriesHead| ==> entriesHead[i].Valid()) {
-        var entry :| entry in entriesHead && !entry.Valid();
-        assert entry in (entriesHead + entriesTail);
-        assert false;
-      }
-    }
-  }
-
-  function method EDKEntryToSeq(edk: Crypto.EncryptedDataKey): seq<uint8>
-    requires edk.Valid()
+  function method EDKEntryToSeq(edk: ESDKEncryptedDataKey): seq<uint8>
   {
     UInt16ToSeq(|edk.keyProviderId| as uint16)   + edk.keyProviderId +
     UInt16ToSeq(|edk.keyProviderInfo| as uint16) + edk.keyProviderInfo +
